zoo_saturn/spmc_queue: Introduce assertions.

theories/zoo_saturn/spmc_queue.v
@@ -1,11 +1,26 @@
+From iris.base_logic Require Import
+  lib.ghost_map.
+
 From zoo Require Import
   prelude.
+From zoo.common Require Import
+  countable
+  list.
+From zoo.iris.bi Require Import
+  big_op.
+From zoo.iris.base_logic Require Import
+  lib.mono_list
+  lib.auth_nat_max
+  lib.auth_twins
+  lib.saved_pred.
 From zoo.language Require Import
   notations.
 From zoo.diaframe Require Import
   diaframe.
 From zoo_std Require Import
-  option.
+  option
+  xtchain
+  domain.
 From zoo_saturn Require Export
   base
   spmc_queue__code.
@@ -14,46 +29,225 @@ From zoo_saturn Require Import
 From zoo Require Import
   options.
 
+Implicit Types b : bool.
+Implicit Types l front node back new_back : location.
+Implicit Types hist past nodes : list location.
 Implicit Types v t : val.
+Implicit Types vs ws : list val.
 
 Class SpmcQueueG Σ `{zoo_G : !ZooG Σ} := {
+  #[local] spmc_queue_G_history_G :: MonoListG Σ location ;
+  #[local] spmc_queue_G_front_G :: AuthNatMaxG Σ ;
+  #[local] spmc_queue_G_model_G :: AuthTwinsG Σ (leibnizO (list val)) suffix ;
+  #[local] spmc_queue_G_waiters_G :: ghost_mapG Σ gname nat ;
+  #[local] spmc_queue_G_saved_pred_G :: SavedPredG Σ bool ;
 }.
 
 Definition spmc_queue_Σ := #[
+  mono_list_Σ location ;
+  auth_nat_max_Σ ;
+  auth_twins_Σ (leibnizO (list val)) suffix ;
+  ghost_mapΣ gname nat ;
+  saved_pred_Σ bool
 ].
 #[global] Instance subG_spmc_queue_Σ Σ `{zoo_G : !ZooG Σ} :
   subG spmc_queue_Σ Σ →
   SpmcQueueG Σ.
 Proof.
-  (* solve_inG. *)
+  solve_inG.
 Qed.
 
 Section spmc_queue_G.
   Context `{spmc_queue_G : SpmcQueueG Σ}.
 
-  Parameter spmc_queue_inv : val → namespace → iProp Σ.
+  Implicit Types Ψ : bool → iProp Σ.
 
-  Parameter spmc_queue_model : val → list val → iProp Σ.
+  Record metadata := {
+    metadata_history : gname ;
+    metadata_front : gname ;
+    metadata_model : auth_twins_name ;
+    metadata_waiters : gname ;
+  }.
+  Implicit Type γ : metadata.
 
-  Parameter spmc_queue_producer : val → list val → iProp Σ.
+  #[local] Instance metadata_eq_dec : EqDecision metadata :=
+    ltac:(solve_decision).
+  #[local] Instance metadata_countable :
+    Countable metadata.
+  Proof.
+    solve_countable.
+  Qed.
+
+  #[local] Definition history_auth' γ_history hist :=
+    mono_list_auth γ_history (DfracOwn (1/2)) hist.
+  #[local] Definition history_auth γ hist :=
+    history_auth' γ.(metadata_history) hist.
+  #[local] Definition history_last' γ_history node : iProp Σ :=
+    ∃ hist,
+    mono_list_auth γ_history (DfracOwn (1/2)) hist ∗
+    ⌜last hist = Some node⌝.
+  #[local] Instance : CustomIpatFormat "history_last" :=
+    "(
+      %hist{} &
+      Hauth{_{}} &
+      %Hlast
+    )".
+  #[local] Definition history_last γ :=
+    history_last' γ.(metadata_history).
+  #[local] Definition history_at γ i node :=
+    mono_list_at γ.(metadata_history) i node.
+
+  #[local] Definition front_auth' γ_front i :=
+    auth_nat_max_auth γ_front (DfracOwn 1) i.
+  #[local] Definition front_auth γ i :=
+    front_auth' γ.(metadata_front) i.
+  #[local] Definition front_lb γ i :=
+    auth_nat_max_lb γ.(metadata_front) i.
+
+  #[local] Definition model₁' γ_model vs :=
+    auth_twins_twin1 _ γ_model vs.
+  #[local] Definition model₁ γ :=
+    model₁' γ.(metadata_model).
+  #[local] Definition model₂' γ_model vs :=
+    auth_twins_twin2 _ γ_model vs.
+  #[local] Definition model₂ γ :=
+    model₂' γ.(metadata_model).
+
+  #[local] Definition producer' γ_model ws :=
+    auth_twins_auth _ γ_model ws.
+  #[local] Definition producer γ :=
+    producer' γ.(metadata_model).
+
+  #[local] Definition waiters_auth' γ_waiters waiters :=
+    ghost_map_auth γ_waiters 1 waiters.
+  #[local] Definition waiters_auth γ waiters :=
+    waiters_auth' γ.(metadata_waiters) waiters.
+  #[local] Definition waiters_at γ waiter i :=
+    ghost_map_elem γ.(metadata_waiters) waiter (DfracOwn 1) i.
+
+  #[local] Definition waiter_au γ ι Ψ : iProp Σ :=
+    AU <{
+      ∃∃ vs,
+      model₁ γ vs
+    }> @ ⊤ ∖ ↑ι, ∅ <{
+      model₁ γ vs
+    , COMM
+      Ψ (bool_decide (vs = []))
+    }>.
+  #[local] Definition waiter_model γ ι past waiter i : iProp Σ :=
+    ∃ Ψ,
+    saved_pred waiter Ψ ∗
+    if decide (i < length past) then
+      Ψ false
+    else
+      waiter_au γ ι Ψ.
+
+  #[local] Definition inv_inner l γ ι : iProp Σ :=
+    ∃ hist past front nodes back vs waiters,
+    ⌜hist = past ++ front :: nodes⌝ ∗
+    ⌜back ∈ hist⌝ ∗
+    l.[front] ↦ #front ∗
+    l.[back] ↦ #back ∗
+    xtchain (Header §Node 2) (DfracOwn 1) hist §Null ∗
+    ([∗ list] node; v ∈ nodes; vs, node.[xtchain_data] ↦ v) ∗
+    history_auth γ hist ∗
+    front_auth γ (length past) ∗
+    model₂ γ vs ∗
+    waiters_auth γ waiters ∗
+    ([∗ map] waiter ↦ i ∈ waiters, waiter_model γ ι past waiter i).
+  #[local] Instance : CustomIpatFormat "inv_inner" :=
+    "(
+      %hist{} &
+      %past{} &
+      %front{} &
+      %nodes{} &
+      %back{} &
+      %vs{} &
+      %waiters{} &
+      >%Hhist{} &
+      >%Hback{} &
+      >Hl_front &
+      >Hl_back &
+      >Hhist &
+      >Hnodes &
+      >Hhistory_auth &
+      >Hfront_auth &
+      >Hmodel₂ &
+      >Hwaiters_auth &
+      Hwaiters
+    )".
+  Definition spmc_queue_inv t ι : iProp Σ :=
+    ∃ l γ,
+    ⌜t = #l⌝ ∗
+    meta l nroot γ ∗
+    inv ι (inv_inner l γ ι).
+  #[local] Instance : CustomIpatFormat "inv" :=
+    "(
+      %l &
+      %γ &
+      -> &
+      #Hmeta &
+      #Hinv
+    )".
+
+  Definition spmc_queue_model t vs : iProp Σ :=
+    ∃ l γ,
+    ⌜t = #l⌝ ∗
+    meta l nroot γ ∗
+    model₁ γ vs.
+  #[local] Instance : CustomIpatFormat "model" :=
+    "(
+      %l_ &
+      %γ_ &
+      %Heq &
+      #Hmeta_ &
+      Hmodel₁
+    )".
+
+  Definition spmc_queue_producer t ws : iProp Σ :=
+    ∃ l γ back,
+    ⌜t = #l⌝ ∗
+    meta l nroot γ ∗
+    l.[back] ↦ #back ∗
+    history_last γ back ∗
+    producer γ ws.
+  #[local] Instance : CustomIpatFormat "producer" :=
+    "(
+      %l{{}=_} &
+      %γ{{}=_} &
+      %Heq{} &
+      #Hmeta_{} &
+      Hmodel₁{}
+    )".
 
   #[global] Instance spmc_queue_model_timeless t vs :
     Timeless (spmc_queue_model t vs).
   Proof.
-  Admitted.
+    apply _.
+  Qed.
   #[global] Instance spmc_queue_producer_timeless t ws :
     Timeless (spmc_queue_producer t ws).
   Proof.
-  Admitted.
+    apply _.
+  Qed.
   #[global] Instance spmc_queue_inv_persistent t ι :
     Persistent (spmc_queue_inv t ι).
   Proof.
-  Admitted.
+    apply _.
+  Qed.
+
+  Opaque history_last'.
 
   Lemma spmc_queue_producer_valid t vs ws :
     spmc_queue_model t vs -∗
     spmc_queue_producer t ws -∗
     ⌜vs `suffix_of` ws⌝.
+  Proof.
+  Admitted.
+  Lemma spmc_queue_producer_exclusive t ws1 ws2 :
+    spmc_queue_producer t ws1 -∗
+    spmc_queue_producer t ws2 -∗
+    False.
   Proof.
   Admitted.
 
@@ -118,11 +312,11 @@ Section spmc_queue_G.
   Admitted.
 End spmc_queue_G.
 
-#[global] Opaque spmc_queue_inv.
-#[global] Opaque spmc_queue_model.
-#[global] Opaque spmc_queue_producer.
-
 #[global] Opaque spmc_queue_create.
 #[global] Opaque spmc_queue_is_empty.
 #[global] Opaque spmc_queue_push.
 #[global] Opaque spmc_queue_pop.
+
+#[global] Opaque spmc_queue_inv.
+#[global] Opaque spmc_queue_model.
+#[global] Opaque spmc_queue_producer.
